\documentclass{article}
\usepackage{amsmath}
\begin{document}
\[
\begin{bmatrix}
    0 & 2 & 3 \\
    8 & 7 & 6 \\
    1 & 4 & 2
\end{bmatrix}
\times
\begin{bmatrix}
    2 & 4 & 1 \\
    7 & 2 & 8 \\
    6 & 3 & 0
\end{bmatrix}
=
\begin{bmatrix}
    33 & 13 & 16 \\
    101 & 64 & 64 \\
    42 & 18 & 33
\end{bmatrix}
\]
\begin{align}
    &(1,1) = 0(2) + 2(7) + 3(6) = 32 \\
    &(1,2) = 0(4) + 2(2) (3)3 = 13 \\
    &(1,3) = 0(1) + 2(8) + 3(0) = 16 \\
    \\
    &(2,1) = 8(2) + 7(7) + 6(6) = 101 \\
    &(2,2) = 8(4) + 7(2) + 6(3) = 64 \\
    &(2,3) = 8(1) + 7(8) + 6(0) = 64 \\
    \\
    &(3,1) = 1(2) + 4(7) + 2(6) = 42 \\
    &(3,2) = 1(4) + 4(2) + 2(3) = 18 \\
    &(3,3) = 1(1) + 4(8) + 2(0) = 33
\end{align}
\end{document}